src/Iris/BI/Updates.lean
@@ -11,12 +11,15 @@ import Iris.BI.DerivedLaws
 import Iris.Algebra
 import Iris.BI.Plainly
 
+namespace Iris
+open Iris.Std BI
+
 --TODO: Which type should we use for sets of masks?
-abbrev Set (α : Type _) := α → Prop
-abbrev setT {α : Type _} : Set α := fun _ => True
-abbrev subset (x y : Set α) : Prop := ∀ a, x a → y a
-abbrev disjoint (x y : Set α) : Prop := ∀ a, ¬(x a ∧ y a)
-abbrev union (x y : Set α) : Set α := fun a => x a ∨ y a
+def Set (α : Type _) := α → Prop
+def Set.univ {α : Type _} : Set α := fun _ => True
+def Subset (x y : Set α) : Prop := ∀ a, x a → y a
+def Disjoint (x y : Set α) : Prop := ∀ a, ¬(x a ∧ y a)
+def union (x y : Set α) : Set α := fun a => x a ∨ y a
 
 class BUpd (PROP : Type _) where
   bupd : PROP → PROP
@@ -24,8 +27,6 @@ export BUpd (bupd)
 
 syntax "|==> " term:40 : term
 syntax term:26 " ==∗ " term:25 : term
-
-open Iris BI
 
 macro_rules
   | `(iprop(|==> $P))  => ``(BUpd.bupd iprop($P))
@@ -53,7 +54,6 @@ macro_rules
 
 -- Delab rules
 
-
 syntax "|={ " term " }[ " term " ]▷=> " term : term
 syntax term "={ " term " }[ " term " ]▷=∗ " term : term
 syntax "|={ " term " }▷=> " term : term
@@ -80,60 +80,55 @@ macro_rules
 
 -- Delab rules
 
-namespace Iris.BI
-open Iris.Std BI
-
-class BiUpdate (PROP : Type _) [BI PROP] extends BUpd PROP where
-  [bupd_nonexpansive : OFE.NonExpansive (BUpd.bupd (PROP := PROP))]
+class BIUpdate (PROP : Type _) [BI PROP] extends BUpd PROP where
+  [bupd_ne : OFE.NonExpansive (BUpd.bupd (PROP := PROP))]
   intro {P : PROP} : iprop(P ⊢ |==> P)
   mono {P Q : PROP} : iprop(P ⊢ Q) → iprop(|==> P ⊢ |==> Q)
   trans {P : PROP} : iprop(|==> |==> P ⊢ |==> P)
   frame_r {P R : PROP} : iprop((|==> P) ∗ R ⊢ |==> (P ∗ R))
 
-class BiFUpdate (PROP MASK : Type _) [BI PROP] extends FUpd PROP MASK where
-  [nonexpansive {E1 E2 : Set MASK} : OFE.NonExpansive (FUpd.fupd E1 E2 (PROP := PROP))]
-  subset {E1 E2 : Set MASK} :
-    subset E2 E1 → iprop(⊢ |={E1, E2}=> |={E2, E1}=> (emp : PROP))
-  except0 {E1 E2 : Set MASK} (P : PROP) :
-    iprop((◇ |={E1, E2}=> P) ⊢ |={E1, E2}=> P)
-  trans {E1 E2 E3 : Set MASK} (P : PROP) :
-    iprop((|={E1, E2}=> |={E2, E3}=> P) ⊢ |={E1, E3}=> P)
+class BIFUpdate (PROP MASK : Type _) [BI PROP] extends FUpd PROP MASK where
+  [ne {E1 E2 : Set MASK} : OFE.NonExpansive (FUpd.fupd E1 E2 (PROP := PROP))]
+  subset {E1 E2 : Set MASK} : Subset E2 E1 → ⊢ |={E1, E2}=> |={E2, E1}=> (emp : PROP)
+  except0 {E1 E2 : Set MASK} (P : PROP) : (◇ |={E1, E2}=> P) ⊢ |={E1, E2}=> P
+  trans {E1 E2 E3 : Set MASK} (P : PROP) : (|={E1, E2}=> |={E2, E3}=> P) ⊢ |={E1, E3}=> P
   mask_frame_r' {E1 E2 Ef : Set MASK} (P : PROP) :
-    disjoint E1 Ef → (|={E1,E2}=> ⌜disjoint E2 Ef⌝ → P) ⊢ |={union E1 Ef, union E2 Ef}=> P
+    Disjoint E1 Ef → (|={E1,E2}=> ⌜Disjoint E2 Ef⌝ → P) ⊢ |={union E1 Ef, union E2 Ef}=> P
   frame_r {E1 E2 : Set MASK} (P R : PROP) :
     iprop((|={E1, E2}=> P) ∗ R ⊢ |={E1, E2}=> P ∗ R)
 
-class BiUpdateFUpdate (PROP : Type _) [BI PROP] [BiUpdate PROP] [BiFUpdate PROP MASK] where
+class BIUpdateFUpdate (PROP : Type _) [BI PROP] [BIUpdate PROP] [BIFUpdate PROP MASK] where
   fupd_of_bupd {P : PROP} {E : Set MASK} : iprop(⊢ |==> P) → iprop(⊢ |={E}=> P)
 
-class BiBUpdatePlainly (PROP : Type _) [BI PROP] [BiUpdate PROP] [BiPlainly PROP] where
+class BIBUpdatePlainly (PROP : Type _) [BI PROP] [BIUpdate PROP] [BIPlainly PROP] where
   bupd_plainly {P : PROP} : iprop((|==> ■ P)) ⊢ P
 
-class BiFUpdatePlainly (PROP MASK : Type _) [BI PROP] [BiFUpdate PROP MASK] [BiPlainly PROP] where
+class BIFUpdatePlainly (PROP MASK : Type _) [BI PROP] [BIFUpdate PROP MASK] [BIPlainly PROP] where
   fupd_plainly_keep_l (E E' : Set MASK) (P R : PROP) : (R ={E,E'}=∗ ■ P) ∗ R ⊢ |={E}=> P ∗ R
   fupd_plainly_later (E : Set MASK) (P : PROP) : (▷ |={E}=> ■ P) ⊢ |={E}=> ▷ ◇ P
-  fupd_plainly_forall_2 (E : Set MASK) {A} (Φ : A → PROP) : (∀ x, |={E}=> ■ Φ x) ⊢ |={E}=> ∀ x, Φ x
+  fupd_plainly_sForall_2 (E : Set MASK) (Φ : PROP → Prop) :
+    (∀ p, ⌜Φ p⌝ → |={E}=> ■ p) ⊢ |={E}=> sForall Φ
 
 section BUpdLaws
 
-variable {PROP : Type _} [BI PROP] [BiUpdate PROP]
+variable [BI PROP] [BIUpdate PROP]
 
-open BI BiUpdate
+open BIUpdate
 
-theorem frame_l {P Q : PROP} : iprop(P ∗ |==> Q ⊢ |==> (P ∗ Q)) :=
+theorem bupd_frame_l {P Q : PROP} : iprop(P ∗ |==> Q ⊢ |==> (P ∗ Q)) :=
   sep_symm.trans <| frame_r.trans <| mono sep_symm
 
-theorem wand_l {P Q : PROP} : iprop((P -∗ Q) ∗ (|==> P) ⊢ |==> Q) :=
-  frame_l.trans <| mono <| wand_elim .rfl
+theorem bupd_wand_l {P Q : PROP} : iprop((P -∗ Q) ∗ (|==> P) ⊢ |==> Q) :=
+  bupd_frame_l.trans <| mono <| wand_elim .rfl
 
-theorem wand_r {P Q : PROP} : iprop((|==> P) ∗ (P -∗ Q) ⊢ |==> Q) :=
-  sep_symm.trans wand_l
+theorem bupd_wand_r {P Q : PROP} : iprop((|==> P) ∗ (P -∗ Q) ⊢ |==> Q) :=
+  sep_symm.trans bupd_wand_l
 
 theorem bupd_sep {P Q : PROP} : iprop((|==> P) ∗ (|==> Q) ⊢ |==> (P ∗ Q)) :=
-  frame_l.trans <| (mono <| frame_r).trans BiUpdate.trans
+  bupd_frame_l.trans <| (mono <| frame_r).trans BIUpdate.trans
 
-theorem idemp {P : PROP} : iprop((|==> |==> P) ⊣⊢ |==> P) :=
-  ⟨BiUpdate.trans, BiUpdate.intro⟩
+theorem bupd_idem {P : PROP} : iprop((|==> |==> P) ⊣⊢ |==> P) :=
+  ⟨BIUpdate.trans, BIUpdate.intro⟩
 
 theorem bupd_or {P Q: PROP} : iprop((|==> P) ∨ (|==> Q) ⊢ |==> (P ∨ Q)) :=
   or_elim (mono or_intro_l) (mono or_intro_r)
@@ -148,18 +143,18 @@ theorem bupd_forall {A : Type} {Φ : A → PROP} :
     iprop(|==> «forall» fun x : A => Φ x) ⊢ «forall» fun x : A => iprop(|==> Φ x) :=
   forall_intro (mono <| forall_elim ·)
 
-theorem bupd_except_0 {P : PROP} : iprop(◇ (|==> P) ⊢ (|==> ◇ P)) :=
+theorem bupd_except0 {P : PROP} : iprop(◇ (|==> P) ⊢ (|==> ◇ P)) :=
   or_elim (or_intro_l.trans intro) (mono or_intro_r)
 
 instance {P : PROP} [Absorbing P] : Absorbing iprop(|==> P) :=
-  ⟨frame_l.trans <| mono <| sep_elim_r⟩
+  ⟨bupd_frame_l.trans <| mono sep_elim_r⟩
 
 section BUpdPlainlyLaws
 
-variable [BiPlainly PROP] [BiBUpdatePlainly PROP]
+variable [BIPlainly PROP] [BIBUpdatePlainly PROP]
 
 theorem bupd_elim {P : PROP} [Plain P] : |==> P ⊢ P :=
-  (mono Plain.plain).trans BiBUpdatePlainly.bupd_plainly
+  (mono Plain.plain).trans BIBUpdatePlainly.bupd_plainly
 
 theorem bupd_plain_forall {A : Type} (Φ : A → PROP) [∀ x, Plain (Φ x)] :
     (|==> ∀ x, Φ x) ⊣⊢ (∀ x, |==> Φ x) := by
@@ -168,7 +163,7 @@ theorem bupd_plain_forall {A : Type} (Φ : A → PROP) [∀ x, Plain (Φ x)] :
   exact (forall_intro fun a => (forall_elim a).trans  bupd_elim)
 
 instance {P : PROP} [Plain P] : Plain iprop(|==> P) :=
-  ⟨(mono Plain.plain).trans <| (bupd_elim).trans <| BiPlainly.mono intro⟩
+  ⟨(mono Plain.plain).trans <| (bupd_elim).trans <| BIPlainly.mono intro⟩
 
 end BUpdPlainlyLaws
 end BUpdLaws
