src/Iris/Instances/UPred/Instance.lean
@@ -15,32 +15,27 @@ open Iris BI
 
 namespace UPred
 
-variable {M : Type} [UCMRA M]
+variable [UCMRA M]
 
 section bidefs
 
-variable (P Q : UPred M)
-variable {A : Type}
-variable {O : Type} [OFE O] (o1 o2 : O)
-variable (m : M)
-
-protected def Entails : Prop := ∀ n x, ✓{n} x → P n x → Q n x
+protected def Entails (P Q : UPred M) : Prop := ∀ n x, ✓{n} x → P n x → Q n x
 
 protected def pure (p : Prop) : UPred M where
   holds _ _ := p
   mono h _ _ := h
 
-protected def and : UPred M where
+protected def and (P Q : UPred M) : UPred M where
   holds n x := P n x ∧ Q n x
   mono HPQ Hle Hn := ⟨P.mono HPQ.1 Hle Hn, Q.mono HPQ.2 Hle Hn⟩
 
-protected def or : UPred M where
+protected def or (P Q : UPred M) : UPred M where
   holds n x := P n x ∨ Q n x
   mono
   | .inl H, Hle, Hn => .inl (P.mono H Hle Hn)
   | .inr H, Hle, Hn => .inr (Q.mono H Hle Hn)
 
-protected def imp : UPred M where
+protected def imp (P Q : UPred M) : UPred M where
   holds n x := ∀ n' x', x ≼ x' → n' ≤ n → ✓{n'} x' → P n' x' → Q n' x'
   mono {n₁ n₂ x₁ x₂} H := fun ⟨m₁, Hle⟩ Hn n x ⟨m₂, Hxle⟩ Hnle Hv HP => by
     have Hx :=
@@ -62,11 +57,11 @@ protected def sExists (Ψ : UPred M → Prop) : UPred M where
   holds n x := ∃ p, Ψ p ∧ p n x
   mono := fun ⟨p, HΨ, Hp⟩ Hv Hn => ⟨p, HΨ, p.mono Hp Hv Hn⟩
 
-protected def eq : UPred M where
+protected def eq [OFE O] (o1 o2 : O) : UPred M where
   holds n _ := o1 ≡{n}≡ o2
   mono H1 _ H2 := H1.le H2
 
-protected def sep : UPred M where
+protected def sep (P Q : UPred M) : UPred M where
   holds n x := ∃ x1 x2, x ≡{n}≡ x1 • x2 ∧ P n x1 ∧ Q n x2
   mono {n₁ n₂ m₁ m₂} := fun ⟨x₁, x₂, Hx, HP, HQ⟩ ⟨m, Hm⟩ Hn => by
     refine ⟨x₁, x₂ • m, ?_, ?_, ?_⟩
@@ -76,7 +71,7 @@ protected def sep : UPred M where
     · exact P.mono HP (CMRA.incN_refl x₁) Hn
     · exact Q.mono HQ (CMRA.incN_op_left n₂ x₂ m) Hn
 
-protected def wand : UPred M where
+protected def wand (P Q : UPred M) : UPred M where
   holds n x := ∀ n' x', n' ≤ n → ✓{n'} (x • x') → P n' x' → Q n' (x • x')
   mono {n₁ n₂ m₁ m₂} H Hm Hn n' x Hn' Hv HP := by
     refine Q.mono ?_ (CMRA.op_monoN_left _ (CMRA.incN_of_incN_le Hn' Hm)) (Nat.le_refl _)
@@ -88,21 +83,21 @@ protected def wand : UPred M where
          _      ≡{n₂}≡ m₁ • (x • y) := CMRA.comm.dist.op_r
          _      ≡{n₂}≡ (m₁ • x) • y := CMRA.assoc.dist
 
-protected def plainly : UPred M where
+protected def plainly (P : UPred M) : UPred M where
   holds n _ := P n UCMRA.unit
   mono H _ Hn := P.mono H (CMRA.incN_refl UCMRA.unit) Hn
 
-protected def persistently : UPred M where
+protected def persistently (P : UPred M) : UPred M where
   holds n x := P n (CMRA.core x)
   mono H Hx Hn := P.mono H (CMRA.core_incN_core Hx) Hn
 
-protected def later : UPred M where
+protected def later (P : UPred M) : UPred M where
   holds n x := match n with | 0 => True | Nat.succ n' => P n' x
   mono {n₁ n₂} := by
     cases n₁ <;> cases n₂ <;> simp
     exact fun H Hx Hn => P.mono H (CMRA.incN_of_incN_succ Hx) Hn
 
-def ownM : UPred M where
+def ownM (m : M) : UPred M where
   holds n x := m ≼{n} x
   mono {n₁ n₂ x₁ x₂} := fun ⟨m₁, Hm₁⟩ ⟨m₂, Hm₂⟩ Hn => by
     exists m₁ • m₂
@@ -113,14 +108,14 @@ def ownM : UPred M where
 instance : OFE.NonExpansive (ownM : M → UPred M) where
   ne _ _ _ H _ _ Hn _ := OFE.Dist.incN (OFE.Dist.le H Hn) .rfl
 
-def validInternal [CMRA A] (a : A): UPred M where
+def validInternal [CMRA A] (a : A) : UPred M where
   holds n _ := ✓{n} a
   mono hv _ le := CMRA.validN_of_le le hv
 
 instance [CMRA A] : OFE.NonExpansive (validInternal : A → UPred M) where
-  ne _ _ _ H _ _ Hn _ := OFE.Dist.validN <| H.le Hn
+  ne _ _ _ H _ _ Hn _ := (H.le Hn).validN
 
-def bupd : UPred M where
+def bupd (Q : UPred M) : UPred M where
   holds n x := ∀ k yf, k ≤ n → ✓{k} (x • yf) → ∃ x', ✓{k} (x' • yf) ∧ Q k x'
   mono {n1 n2} {x1 x2} HQ := by
     rintro ⟨x3, Hx⟩ Hn k yf Hk Hx0
@@ -363,103 +358,51 @@ instance : OFE.NonExpansive (plainly : UPred M → UPred M) where
     · exact uPred_holds_ne (HP.symm.le Hn') n'.le_refl CMRA.unit_validN
     · exact uPred_holds_ne (HP.le Hn') n'.le_refl CMRA.unit_validN
 
-theorem plainly_mono {P Q : UPred M} (H : P ⊢ Q) : ■ P ⊢ ■ Q :=
-  fun _ _ _ => H _ _ CMRA.unit_validN
-
-theorem plainly_elim_persistently {P : UPred M} : ■ P ⊢ <pers> P := by
-  intro n x Hx; simp [plainly, UPred.plainly]; intro H
-  refine iprop(<pers> P).mono ?_ CMRA.incN_unit n.le_refl
-  simp [intuitionistically, affinely, UPred.persistently, persistently, BIBase.and, UPred.and]
-  exact P.mono H CMRA.incN_unit n.le_refl
-
-theorem plainly_idemp_2 {P : UPred M} : ■ P ⊢ ■ ■ P :=
-  fun _ _ _ H => H
-
-theorem plainly_forall_2 {A : Type} {Ψ : A → UPred M} : (∀ a, ■ Ψ a) ⊢ (■ «forall» fun a => iprop(Ψ a)) := by
-  intro _ _ _
-  simp [plainly, UPred.plainly, BIBase.forall, sForall, UPred.sForall]
-
-theorem plainly_exist_1 {A : Type} {Ψ : A → UPred M} : (■ ∃ a, Ψ a) ⊢ («exists» fun a => iprop(■ Ψ a)) := by
-  intro n x Hx
-  simp [plainly, UPred.plainly, BIBase.exists, sExists, UPred.sExists]
-  intro a HA
-  exists iprop(■ Ψ a)
-  refine ⟨⟨a, rfl⟩, (Ψ a).mono HA CMRA.incN_unit n.le_refl⟩
-
-theorem plainly_emp_intro {P : UPred M} : P ⊢ ■ emp := fun _ _ _ _ => trivial
-
-theorem plainly_absorb {P Q : UPred M}: ■ P ∗ Q ⊢ ■ P  := sep_elim_l
-
-theorem persistently_impl_plainly {P Q : UPred M} : (■ P → <pers> Q) ⊢ <pers> (■ P → Q) := by
-  intro n x Hx HPQ n' x' Hx' Hn Hv H
-  apply Q.mono _ (CMRA.incN_of_inc _ Hx') n'.le_refl
-  apply HPQ _ _ CMRA.Included.rfl Hn (CMRA.validN_of_le Hn Hx)
-  exact H
-
-
-theorem plainly_impl_plainly {P Q : UPred M} : (■ P → ■ Q) ⊢ ■ (■ P → Q) := by
-  intro n x Hx HPQ n' x' Hx' Hn Hv H
-  apply Q.mono _ (CMRA.incN_of_inc _ Hx') n'.le_refl
-  apply HPQ _ _ CMRA.Included.rfl Hn (CMRA.validN_of_le Hn Hx)
-  exact H
-
-instance : BiPlainly (UPred M) where
-  mono := plainly_mono
-  elim_persistently := plainly_elim_persistently
-  idemp := plainly_idemp_2
-  plainly_forall_2 := plainly_forall_2
-  plainly_impl_plainly := plainly_impl_plainly
-  emp_intro := plainly_emp_intro
-  plainly_absorb := plainly_absorb
+instance : BIPlainly (UPred M) where
+  mono H _ _ _ := H _ _ CMRA.unit_validN
+  elim_persistently {P} n x Hx := by
+    simp [plainly, UPred.plainly]; intro H
+    refine iprop(<pers> P).mono ?_ CMRA.incN_unit n.le_refl
+    simp [intuitionistically, affinely, UPred.persistently, persistently, BIBase.and, UPred.and]
+    exact P.mono H CMRA.incN_unit n.le_refl
+  idem _ _ _ := id
+  plainly_sForall_2 _ _ hv H _ := H _ ⟨_, rfl⟩ _ _ .rfl (Nat.le_refl _) hv
+  plainly_impl_plainly {P Q} n x Hx HPQ n' x' Hx' Hn Hv H := by
+    apply Q.mono _ (CMRA.incN_of_inc _ Hx') n'.le_refl
+    apply HPQ _ _ CMRA.Included.rfl Hn (CMRA.validN_of_le Hn Hx)
+    exact H
+  emp_intro _ _ _ _ := trivial
+  plainly_absorb := sep_elim_l
   later_plainly := ⟨Std.refl, Std.refl⟩
 
-instance : BiPlainlyExist (UPred M) where
-  plainly_exist_1 := plainly_exist_1
+instance : BIPlainlyExists (UPred M) where
+  plainly_sExists_1 _ _ _ := fun ⟨_, hp⟩ => ⟨_, ⟨_, rfl⟩, hp⟩
 
 instance : BUpd (UPred M) := ⟨bupd⟩
 
-theorem bupd_intro {P : UPred M} : P ⊢ |==> P :=
-  fun _ x _ HP _ _ Hn H => ⟨_, ⟨H, P.mono HP (CMRA.incN_refl x) Hn⟩⟩
+instance : OFE.NonExpansive (BUpd.bupd (PROP := UPred M)) := bupd_ne
 
-theorem bupd_mono {P Q : UPred M} : (P ⊢ Q) → (|==> P) ⊢ |==> Q := by
-  intros Himp n x Hx HP k yf Hn H
-  rcases HP k yf Hn H with ⟨x', Hx'⟩
-  refine ⟨x', ⟨Hx'.1, Himp _ _ ?_ Hx'.2⟩⟩
-  exact CMRA.validN_op_left Hx'.1
+instance : BIUpdate (UPred M) where
+  intro {P} _ x _ HP _ _ Hn H := ⟨_, ⟨H, P.mono HP (CMRA.incN_refl x) Hn⟩⟩
+  mono Himp n x Hx HP k yf Hn H := by
+    rcases HP k yf Hn H with ⟨x', Hx'⟩
+    refine ⟨x', ⟨Hx'.1, Himp _ _ ?_ Hx'.2⟩⟩
+    exact CMRA.validN_op_left Hx'.1
+  trans n x Hx H k yf Hx Hyf :=
+    let ⟨x', Hx', Hx''⟩ := H k yf Hx Hyf
+    Hx'' k yf k.le_refl Hx'
+  frame_r {P R} n x Hx := fun ⟨x1, x2, Hx, HP, HR⟩ k yf Hk Hyf => by
+    have L : ✓{k} x1 • (x2 • yf) :=
+      (CMRA.op_assocN.trans (Hx.le Hk).op_l.symm).validN.2 Hyf
+    let ⟨x', Hx'1, Hx'2⟩ := HP k (x2 • yf) Hk L
+    refine ⟨x' • x2, CMRA.op_assocN.validN.1 Hx'1, x', x2, .rfl, Hx'2, ?_⟩
+    exact R.mono HR (CMRA.incN_refl x2) Hk
 
-theorem bupd_trans {P : UPred M} : (|==> |==> P) ⊢ |==> P := by
-  intro n x Hx H k yf Hx Hyf
-  rcases H k yf Hx Hyf with ⟨x', ⟨Hx', Hx''⟩⟩
-  exact Hx'' k yf k.le_refl Hx'
-
-theorem bupd_frame_r {P R : UPred M} : (|==> P) ∗ R ⊢ |==> (P ∗ R) := by
-  rintro n x Hx ⟨x1, x2, Hx, HP, HR⟩ k yf Hk Hyf
-  have L : ✓{k} x1 • (x2 • yf) := by
-    refine CMRA.validN_ne CMRA.op_assocN.symm ?_
-    refine CMRA.validN_ne ?_ Hyf
-    exact CMRA.op_left_dist _ (OFE.Dist.le Hx Hk)
-  rcases HP k (x2 • yf) Hk L with ⟨x', Hx'1, Hx'2⟩
-  refine ⟨x' • x2, ⟨CMRA.validN_ne CMRA.op_assocN Hx'1, ?_⟩⟩
-  refine ⟨x', ⟨x2, ⟨OFE.Dist.rfl, ⟨Hx'2, ?_⟩⟩⟩⟩
-  exact R.mono HR (CMRA.incN_refl x2) Hk
-
- theorem bupd_plainly {P : UPred M} : (|==> ■ P) ⊢ P := by
-   intro n x Hx Hv
-   simp [bupd, plainly, UPred.plainly, UPred.bupd, BUpd.bupd] at Hv
-   have L : ✓{n} x • UCMRA.unit := CMRA.validN_ne (OFE.equiv_dist.mp CMRA.unit_right_id.symm _) Hx
-   rcases Hv n CMRA.unit n.le_refl L with ⟨x', Hx'⟩
-   apply P.mono Hx' CMRA.incN_unit n.le_refl
-
-instance : BiUpdate (UPred M) where
-  -- FIXME: Why don't you infer?
-  bupd_nonexpansive := bupd_ne
-  intro := bupd_intro
-  mono := bupd_mono
-  trans := bupd_trans
-  frame_r := bupd_frame_r
-
-instance : BiBUpdatePlainly (UPred M) where
-  bupd_plainly := bupd_plainly
+instance : BIBUpdatePlainly (UPred M) where
+  bupd_plainly {P} n x Hx Hv := by
+    have L : ✓{n} x • CMRA.unit := CMRA.unit_right_id.symm.dist.validN.1 Hx
+    let ⟨x', _, Hx'⟩ := Hv n CMRA.unit n.le_refl L
+    exact P.mono Hx' CMRA.incN_unit n.le_refl
 
 theorem ownM_valid (m : M) : ownM m ⊢ validInternal m := fun _ _ h hp => hp.validN h
 
@@ -494,10 +437,12 @@ theorem validInternal_intro [CMRA A] {P : UPred M} (a : A) (Ha : ✓ a) : P ⊢ 
 theorem validInternal_elim [CMRA A] (a : A) : (validInternal a : UPred M) ⊢ iprop(⌜ ✓{0} a ⌝) :=
   fun n _ _ H => CMRA.validN_of_le n.zero_le H
 
-theorem plainly_cmra_validInternal_1 [CMRA A] (a : A) : (validInternal a : UPred M) ⊢ ■ validInternal a :=
+theorem plainly_cmra_validInternal_1 [CMRA A] (a : A) :
+    (validInternal a : UPred M) ⊢ ■ validInternal a :=
   Std.refl
 
-theorem cmra_validInternal_weaken [CMRA A] (a b : A) : (validInternal (a • b) : UPred M) ⊢ validInternal a :=
+theorem cmra_validInternal_weaken [CMRA A] (a b : A) :
+    (validInternal (a • b) : UPred M) ⊢ validInternal a :=
   fun _ _ _ H => CMRA.validN_op_left H
 
 theorem validInternal_entails [CMRA A] [CMRA B] {a : A} {b : B} (Hv : ∀ n, ✓{n} a → ✓{n} b) :
